wip

HumanEvalLean/HumanEval129.lean
@@ -1,5 +1,308 @@
-def minPath : Unit :=
-  ()
+module
+
+import Std
+import all Init.Data.Range.Polymorphic.RangeIterator
+open Std Std.Do
+
+def Vector.iter (xs : Vector α n) :=
+    (xs.toArray.iter : Iter α)
+
+@[simp, grind =]
+theorem Vector.toList_iter {xs : Vector α n} :
+    xs.iter.toList = xs.toList := by
+  simp [Vector.iter, Vector.toList_toArray]
+
+@[simp, grind =]
+theorem Vector.count_iter {xs : Vector α n} :
+    xs.iter.count = n := by
+  simp [Vector.iter, ← Iter.size_toArray_eq_count]
+
+/-
+Zip restructuring plan:
+
+* have zipWith
+* provide proof that there's an i s.t. x = it₁.atIdxSlow? i ∧ y = it₂.atIdxSlow? i ∧
+-/
+
+def Std.Iter.enumerate [Iterator α Id β] (it : Iter (α := α) β) :=
+  (it.zip (*...* : Std.Rii Nat).iter : Iter (β × Nat))
+
+instance [Iterator α Id β] [Iterators.Productive α Id] : Membership β (Iter (α := α) β) where
+  mem it x := ∃ n : Nat, it.atIdxSlow? n = some x
+
+theorem Std.Iter.mem_toList_iff [Iterator α Id β] [Iterators.Finite α Id]
+    {it : Iter (α := α) β} {x : β} :
+    x ∈ it.toList ↔ x ∈ it := by
+  sorry
+
+theorem Std.Iter.atIdxSlow?_eq_getElem?_toList_take {α β} [Iterator α Id β] [Iterators.Productive α Id]
+    {it : Iter (α := α) β} {k : Nat} :
+    it.atIdxSlow? k = (it.take (k + 1)).toList[k]? := by
+  fun_induction it.atIdxSlow? k with
+  | case1 it _ _ _ h
+  | case2 it _ _ _ _ _ h
+  | case3 _ it _ _ h
+  | case4 _ it _ h =>
+    rw [Iter.toList_eq_match_step, Iter.step_take, h]
+    cases _ : it.step using PlausibleIterStep.casesOn <;> grind
+
+theorem Std.Iter.mem_zip_iff [Iterator α₁ Id β₁] [Iterator α₂ Id β₂]
+    [Iterators.Productive α₁ Id] [Iterators.Productive α₂ Id]
+    {it₁ : Iter (α := α₁) β₁} {it₂ : Iter (α := α₂) β₂} {p : β₁ × β₂} :
+    p ∈ it₁.zip it₂ ↔ ∃ n, it₁.atIdxSlow? n = some p.1 ∧ it₂.atIdxSlow? n = some p.2 := by
+  simp only [Membership.mem, atIdxSlow?_zip]
+  apply Iff.intro
+  · rintro ⟨n, h⟩
+    cases h₁ : it₁.atIdxSlow? n <;> cases h₂ : it₂.atIdxSlow? n <;> grind
+  · rintro ⟨n, h₁, h₂⟩
+    cases h₁ : it₁.atIdxSlow? n <;> cases h₂ : it₂.atIdxSlow? n <;> grind
+
+-- TODO: remove `Nat.toList_rio_zero_right_eq_nil`
+@[grind =]
+theorem Nat.toList_rio_zero :
+    (*...0).toList = [] := by
+  simp
+
+theorem Nat.toList_take_add_one_iter_rci {m n : Nat} :
+    ((m...*).iter.take (n + 1)).toList = m :: (((m + 1)...*).iter.take n).toList := by
+  rw [Iter.toList_eq_match_step, Iter.step_take]
+  simp only [Std.Rxi.Iterator.step_eq_step, Rxi.Iterator.step_eq_monadicStep, Rxi.Iterator.Monadic.step]
+  dsimp only [Std.Rci.iter, Iter.toIterM]
+  simp [PRange.Nat.succ?_eq, IterStep.mapIterator_yield, PlausibleIterStep.yield, IterM.toIter]
+
+theorem Nat.toList_take_iter_rci {m n : Nat} :
+    ((m...*).iter.take n).toList = (m...(m + n)).toList := by
+  induction n generalizing m
+  · grind [Iter.toList_take_zero, toList_rco_eq_nil]
+  · rename_i n ih
+    rw [Nat.toList_rco_eq_cons (by grind)]
+    grind [Nat.toList_take_add_one_iter_rci]
+
+theorem Nat.toList_take_iter_rii {n : Nat} :
+    ((*...* : Std.Rii Nat).iter.take n).toList = (*...n).toList := by
+  simpa using Nat.toList_take_iter_rci (m := 0) (n := n)
+
+theorem Std.Iter.mem_enumerate_iff [Iterator α Id β]
+    [Iterators.Finite α Id] {it : Iter (α := α) β}
+    {p : β × Nat} :
+    p ∈ it.enumerate ↔ it.atIdxSlow? p.2 = some p.1 := by
+  simp only [enumerate, mem_zip_iff, ← getElem?_toList_eq_atIdxSlow?,
+    atIdxSlow?_eq_getElem?_toList_take, Nat.toList_take_iter_rii, Nat.getElem?_toList_rio_eq_some_iff]
+  grind
+
+theorem Vector.mem_iter_iff {xs : Vector α n} {x : α} :
+    x ∈ xs.iter ↔ x ∈ xs := by
+  sorry
+
+theorem Vector.atIdxSlow?_iter {xs : Vector α n} {i : Nat} :
+    xs.iter.atIdxSlow? i = xs[i]? := by
+  sorry
+
+theorem Vector.mem_enumerate_iter_iff {xs : Vector α n} {p : α × Nat} :
+    p ∈ xs.iter.enumerate ↔ ∃ (h : p.2 < n), xs[p.2] = p.1 := by
+  rw [Iter.mem_enumerate_iff, Vector.atIdxSlow?_iter]
+  grind
+
+theorem Std.Iter.lt_count_of_mem_enumerate [Iterator α Id β]
+    [IteratorLoop α Id Id] [LawfulIteratorLoop α Id Id]
+    [Iterators.Finite α Id] {it : Iter (α := α) β} {p : β × Nat}
+    (h : p ∈ it.enumerate) :
+    p.2 < it.count := by
+  simp only [enumerate] at h
+  simp only [mem_zip_iff] at h
+  simp only [← getElem?_toList_eq_atIdxSlow?] at h
+  obtain ⟨n, hn, h⟩ := h
+  simp only [List.getElem?_eq_some_iff] at hn
+  obtain ⟨hn, _⟩ := hn
+  simp only [atIdxSlow?_eq_getElem?_toList_take] at h
+  grind [length_toList_eq_count, Nat.getElem_toList_rio, Nat.toList_take_iter_rii]
+
+theorem Std.Iter.mem_of_mem_enumerate [Iterator α Id β] [Iterators.Productive α Id]
+    {it : Iter (α := α) β} {p : β × Nat} (h : p ∈ it.enumerate) :
+    p.1 ∈ it := by
+  simp only [enumerate, mem_zip_iff] at h
+  obtain ⟨n, hn, _⟩ := h
+  exact ⟨n, hn⟩
+
+theorem Std.Iter.toList_enumerate [Iterator α Id β] [Iterators.Finite α Id] (it : Iter (α := α) β) :
+    it.enumerate.toList = it.toList.zipIdx := by
+  simp only [enumerate, toList_zip_of_finite_left, Nat.toList_take_iter_rii, Nat.toList_rio_eq_toList_rco, ← List.range_eq_toList_rco]
+  simp only [List.zipIdx_eq_zip_range', List.range_eq_range']
+
+def WFGrid (grid : Vector (Vector Nat n) n) : Prop :=
+  grid.flatten.toList.Perm (1...=(n * n)).toList
+
+theorem List.isSome_findSome? {xs : List α} {f : α → Option β} :
+    (xs.findSome? f).isSome = xs.any (f · |>.isSome) := by
+  rw [Bool.eq_iff_iff]
+  simp only [Option.isSome_iff_ne_none, ne_eq, findSome?_eq_none_iff, Classical.not_forall]
+  simp only [← Option.isSome_iff_ne_none]
+  grind
+
+def coordsOf? (grid : Vector (Vector Nat n) m) (l : Nat) : Option (Nat × Nat) :=
+    grid.iter.enumerate.findSome? (fun (row, x) =>
+        row.iter.enumerate.findSome? (fun (cell, y) =>
+            if cell = l then some (x, y) else none))
+
+theorem isSome_coordsOf?_one {grid : Vector (Vector Nat n) n} (hn : 0 < n) (h : WFGrid grid) :
+    (coordsOf? grid 1).isSome := by
+  simp only [WFGrid] at h
+  simp only [coordsOf?, ← Iter.findSome?_toList, Iter.toList_enumerate, Vector.toList_iter]
+  simp only [List.isSome_findSome?]
+  have : 1 ∈ grid.flatten.toList := h.mem_iff.mpr (by simp [Std.Rcc.mem_toList_iff_mem, Std.Rcc.mem_iff]; grind [Nat.le_mul_self n])
+  simp [Vector.flatten, Vector.toList_toArray] at this
+  obtain ⟨l, ⟨⟨col, h_col_mem, heq⟩, h_one_mem⟩⟩ := this
+  simp only [Vector.mem_iff_getElem] at h_col_mem
+  obtain ⟨x, hx, hcol⟩ := h_col_mem
+  simp only [List.mem_iff_getElem] at h_one_mem
+  obtain ⟨y, hy, hcell⟩ := h_one_mem
+  simp only [List.any_eq_true, List.mem_zipIdx_iff_getElem?]
+  exact ⟨⟨col, x⟩, by grind, ⟨1, y⟩, by grind⟩
+
+@[grind →]
+theorem coordsOf?_spec {grid : Vector (Vector Nat n) m} {l : Nat} {x y : Nat}
+    (h : coordsOf? grid l = some (x, y)) :
+    ∃ (_ : x < m) (_ : y < n), grid[x][y] = l := by
+  simp only [coordsOf?] at h
+  simp only [← Iter.findSome?_toList] at h
+  obtain ⟨⟨row, x'⟩, h₁, h⟩ := List.exists_of_findSome?_eq_some h
+  simp only [Iter.mem_toList_iff, Vector.mem_enumerate_iter_iff] at h₁
+  obtain ⟨hx, hrow⟩ := h₁
+  obtain ⟨y', h₂, h⟩ := List.exists_of_findSome?_eq_some h
+  simp only [Iter.mem_toList_iff, Vector.mem_enumerate_iter_iff] at h₂
+  obtain ⟨hy, hcell⟩ := h₂
+  grind
+
+def leastNeighborValue (grid : Vector (Vector Nat n) m) (x y : Nat)
+    (hxy : x < m ∧ y < n := by grind) : Nat := Id.run do
+    let mut val := n * n + 1
+    if 0 < x then
+      val := min val grid[x - 1][y]
+    if 0 < y then
+      val := min val grid[x][y - 1]
+    if hx : x + 1 < m then
+      val := min val grid[x + 1][y]
+    if hy : y + 1 < n then
+      val := min val grid[x][y + 1]
+    return val
+
+def minPath (grid : Vector (Vector Nat n) n) (k : Nat) : List Nat := Id.run do
+  match h : coordsOf? grid 1 with
+  | none => return []
+  | some (x, y) =>
+    let val := leastNeighborValue grid x y
+    let mut result := if k % 2 = 1 then [1] else []
+    for _ in *...(k / 2) do
+      result := 1 :: val :: result
+    return result
+
+theorem length_minPath {grid : Vector (Vector Nat n) n} {k : Nat} (hn : 0 < n) (h : WFGrid grid) :
+    (minPath grid k).length = k := by
+  generalize hwp : minPath grid k = wp
+  apply Id.of_wp_run_eq hwp
+  mvcgen +jp -- fails if `coordsOf? grid 1` is extracted into `let bla := ...`
+  invariants
+  · ⇓⟨cur, xs⟩ => ⌜xs.length = if k % 2 = 1 then 2 * cur.pos + 1 else 2 * cur.pos⌝
+  with grind [isSome_coordsOf?_one, Rio.length_toList, Nat.size_rio]
+
+theorem getElem_minPath_eq_one {grid : Vector (Vector Nat n) n} {k : Nat}
+    {i : Nat} {h : i < (minPath grid k).length} (hi : i % 2 = 0) :
+    (minPath grid k)[i]'h = 1 := by
+  simp only [List.getElem_eq_iff]
+  revert i
+  generalize hwp : minPath grid k = wp
+  apply Id.of_wp_run_eq hwp
+  mvcgen +jp -- fails if `coordsOf? grid 1` is extracted into `let bla := ...`
+  invariants
+  · ⇓⟨cur, xs⟩ => ⌜∀ j (hj : j < xs.length), j % 2 = 0 → xs[j] = 1⌝
+  with grind
+
+theorem getElem_minPath_of_odd {grid : Vector (Vector Nat n) n} {k : Nat} (hn : 1 < n)
+    (hg : WFGrid grid)
+    {i : Nat} {h : i < (minPath grid k).length} (hi : i % 2 = 1) :
+    let coords := (coordsOf? grid 1).get (isSome_coordsOf?_one (by grind) hg)
+    have := coordsOf?_spec (Option.some_get (isSome_coordsOf?_one (by grind) hg)).symm
+    let val := (leastNeighborValue grid coords.1 coords.2 (by grind))
+    (minPath grid k)[i]'h = val := by
+  intro coords _ val
+  simp only [List.getElem_eq_iff]
+  revert i
+  generalize hwf : minPath grid k = wf
+  apply Id.of_wp_run_eq hwf
+  mvcgen
+  invariants
+  · ⇓⟨cur, xs⟩ => ⌜∀ j (hj : j < xs.length), j % 2 = 1 → xs[j] = val⌝
+  with grind
+
+inductive AreNeighbors : (p q : Nat × Nat) → Prop
+  | left : AreNeighbors (x + 1, y) (x, y)
+  | right : AreNeighbors (x, y) (x + 1, y)
+  | up : AreNeighbors (x, y) (x, y + 1)
+  | down : AreNeighbors (x, y + 1) (x, y)
+
+@[grind .]
+theorem AreNeighbors.left_of_pos {x y : Nat} (h : 0 < x) :
+    AreNeighbors (x, y) (x - 1, y) := by
+  have := AreNeighbors.left (x := x - 1) (y := y)
+  grind
+
+@[grind .]
+theorem AreNeighbors.down_of_pos {x y : Nat} (h : 0 < y) :
+    AreNeighbors (x, y) (x, y - 1) := by
+  have := AreNeighbors.down (x := x) (y := y - 1)
+  grind
+
+attribute [grind .] AreNeighbors.right AreNeighbors.up
+
+-- def IsInGrid (n : Nat) (p : Nat × Nat) : Prop :=
+--     p.1 < n ∧ p.2 < n
+
+theorem exists_areNeighbors {p : Nat × Nat} (hn : 1 < n) (hxn : p.1 < n) (hyn : p.2 < n) :
+    ∃ q, q.1 < n ∧ q.2 < n ∧ AreNeighbors p q := by
+  by_cases hx : 0 < p.1
+  · have := AreNeighbors.left (x := p.1 - 1) (y := p.2)
+    exact ⟨(p.1 - 1, p.2), by grind⟩
+  · have := AreNeighbors.right (x := p.1) (y := p.2)
+    exact ⟨(p.1 + 1, p.2), by grind⟩
+
+theorem le_leastNeighborValue_iff {grid : Vector (Vector Nat n) n} {x y : Nat}
+    (hn : 1 < n) (hg : WFGrid grid) (hx : x < n) (hy : y < n) :
+    k ≤ leastNeighborValue grid x y ↔ ∀ x' y' (_ : x' < n) (_ : y' < n), AreNeighbors (x, y) (x', y') → k ≤ grid[x'][y'] := by
+  generalize hwp : leastNeighborValue grid x y = wp
+  apply Id.of_wp_run_eq hwp
+  mvcgen +jp
+  rename_i val₀ _ val₁ _ _ val₂ _ _ val₃ _ _ val₄ _ h₁ h₂ h₃ h₄
+  apply Iff.intro
+  · intro h x' y' hx' hy' hnb
+    cases hnb <;> grind
+  · intro h
+    obtain ⟨⟨x', y'⟩, hx', hy', h'⟩ := exists_areNeighbors (p := (x, y)) hn hx hy
+    have hsq := h x' y' hx' hy' h'
+    have : grid[x'][y'] < n * n + 1 := by
+      have : grid[x'][y'] ∈ (1...=(n * n)).toList := hg.mem_iff.mp (by simp [Vector.mem_flatten]; simp only [Vector.mem_iff_getElem]; grind)
+      simp only [Std.Rcc.mem_iff, Std.Rcc.mem_toList_iff_mem] at this
+      grind
+    have : k ≤ val₀ := by grind
+    have : k ≤ val₁ := by split at h₁ <;> (simp only [h₁, le_min_iff]; grind)
+    have : k ≤ val₂ := by split at h₂ <;> (simp only [h₂, le_min_iff]; grind)
+    have : k ≤ val₃ := by split at h₃ <;> (simp only [h₃, le_min_iff]; grind)
+    split at h₄ <;> (simp only [h₄, le_min_iff]; grind)
+
+theorem areNeighbors_minPath {grid : Vector (Vector Nat n) n} {k i : Nat}
+    (hn : 1 < n) (hg : WFGrid grid) (hi : i + 1 < k) :
+    ∃ (p q : Nat × Nat) (_ : p.1 < n) (_ : p.2 < n) (_ : q.1 < n) (_ : q.2 < n),
+      AreNeighbors p q ∧
+      grid[p.1][p.2] = (minPath grid k)[i]! ∧
+      grid[q.1][q.2] = (minPath grid k)[i + 1]! := by
+  by_cases h : i % 2 = 0
+  · let coordsOfFst := (coordsOf? grid 1).get!
+    refine ⟨coordsOfFst, ?_⟩
+    let coordsOfSnd :=
+    conv =>
+      congr; ext p; congr; ext q; congr; ext; congr; ext; congr; ext; congr; ext
+      rw [getElem_minPath_eq_one h, getElem_minPath_of_odd (by grind) hg (by grind)]
+    sorry
+
 
 /-!
 ## Prompt
@@ -8,7 +311,7 @@ def minPath : Unit :=
 
 def minPath(grid, k):
     """
-    Given a grid with N rows and N columns (N >= 2) and a positive integer k, 
+    Given a grid with N rows and N columns (N >= 2) and a positive integer k,
     each cell of the grid contains a value. Every integer in the range [1, N * N]
     inclusive appears exactly once on the cells of the grid.
 
